src/Transcription/Completeness.v
@@ -1,0 +1,206 @@
+From Coq Require Import List.
+
+From compcert Require Import common.Errors.
+From Velus Require Import Common.
+From Velus Require Import Environment.
+From Velus Require Import Operators.
+From Velus Require Import Clocks.
+From Velus Require Import CoindStreams.
+
+From Velus Require Import Lustre.LSyntax.
+From Velus Require Import Lustre.LTyping.
+From Velus Require Import Lustre.LClocking.
+From Velus Require Import Lustre.LOrdered.
+From Velus Require Import Lustre.LSemantics.
+From Velus Require Import Lustre.LNormalization.
+
+From Velus Require Import CoreExpr.CESyntax.
+From Velus Require Import NLustre.NLSyntax.
+From Velus Require Import Transcription.Transcription.
+
+Module Type COMPLETENESS
+       (Import Ids : IDS)
+       (Import Op : OPERATORS)
+       (Import OpAux : OPERATORS_AUX Op)
+       (Str  : COINDSTREAMS Op OpAux)
+       (Import LSyn : LSYNTAX Ids Op)
+       (LTyp : LTYPING Ids Op LSyn)
+       (LOrd : LORDERED Ids Op LSyn)
+       (LSem : LSEMANTICS Ids Op OpAux LSyn LOrd Str)
+       (Import LNorm : LNORMALIZATION Ids Op OpAux Str LSyn LTyp LOrd LSem)
+       (Import CE : CESYNTAX Op)
+       (NL : NLSYNTAX Ids Op CE)
+       (Import TR : TRANSCRIPTION Ids Op OpAux LSyn CE NL).
+
+  Fact to_constant_complete : forall c,
+    is_constant c ->
+    exists e', to_constant c = OK e'.
+  Proof with eauto.
+    intros c Hnorm. induction Hnorm.
+    - eexists; simpl...
+    - destruct IHHnorm as [e' He'].
+      eexists; simpl...
+  Qed.
+
+  Fact to_lexp_complete : forall e,
+    normalized_lexp e ->
+    exists e', to_lexp e = OK e'.
+  Proof with eauto.
+    intros e Hnorm.
+    induction e using exp_ind2; inv Hnorm.
+    - (* const *) eexists; simpl...
+    - (* var *) eexists; simpl...
+    - (* unop *)
+      apply IHe in H0. destruct H0 as [e' He'].
+      eexists; simpl.
+      rewrite He'; simpl...
+    - (* binop *)
+      apply IHe1 in H1. destruct H1 as [e1' He1].
+      apply IHe2 in H4. destruct H4 as [e2' He2].
+      eexists; simpl.
+      rewrite He1. rewrite He2. simpl...
+    - (* when *)
+      inv H. apply H3 in H1. destruct H1 as [e' He'].
+      eexists; simpl.
+      rewrite He'. simpl...
+  Qed.
+
+  Corollary mmap_to_lexp_complete : forall es,
+      Forall normalized_lexp es ->
+      exists es', mmap to_lexp es = OK es'.
+  Proof with eauto.
+    intros es Hf.
+    induction Hf.
+    - eexists; simpl...
+    - apply to_lexp_complete in H.
+      destruct H as [e' He']. destruct IHHf as [es' Hes'].
+      eexists; simpl.
+      rewrite He'; rewrite Hes'. simpl...
+  Qed.
+
+  Fact to_cexp_complete : forall e,
+      normalized_cexp e ->
+      exists e', to_cexp e = OK e'.
+  Proof with eauto.
+    intros e Hnorm.
+    induction e using exp_ind2; inv Hnorm;
+      try (eapply to_lexp_complete in H; destruct H as [e' He'];
+           exists (Eexp e'); unfold to_cexp; rewrite He'; simpl; eauto);
+      try (solve [inv H1]).
+    - (* when *)
+      eapply to_lexp_complete in H0. destruct H0 as [e' He'].
+      exists (Eexp e'). unfold to_cexp. rewrite He'; simpl...
+    - (* merge *)
+      inv H. inv H0.
+      apply H4 in H3. destruct H3 as [et' Het'].
+      apply H2 in H6. destruct H6 as [ef' Hef'].
+      eexists. simpl.
+      rewrite Het'. rewrite Hef'. simpl...
+    - (* ite *)
+      inv H. inv H0.
+      apply to_lexp_complete in H4. destruct H4 as [e' He'].
+      apply H3 in H6. destruct H6 as [et' Het'].
+      apply H2 in H7. destruct H7 as [ef' Hef'].
+      eexists; simpl.
+      rewrite He'. rewrite Het'. rewrite Hef'. simpl...
+  Qed.
+
+  Fact to_equation_complete : forall xs es out env envo,
+      normalized_equation out (xs, es) ->
+      Forall (fun x => exists cl, find_clock env x = OK cl) xs ->
+      (forall x e, envo x = Error e -> In x out) ->
+      exists eq', to_equation env envo (xs, es) = OK eq'.
+  Proof with eauto.
+    intros xs es out env envo Hnorm Hfind Henvo.
+    inv Hnorm.
+    - apply mmap_to_lexp_complete in H1. destruct H1 as [es' Hes'].
+      eexists; simpl. rewrite Hes'; simpl...
+    - apply mmap_to_lexp_complete in H1. destruct H1 as [es' Hes'].
+      destruct cl.
+      eexists; simpl. rewrite Hes'. simpl...
+    - apply to_constant_complete in H3. destruct H3 as [e0' He0'].
+      apply to_lexp_complete in H4. destruct H4 as [e' He'].
+      inv Hfind. destruct H2 as [cl Hcl].
+      eexists; simpl.
+      rewrite He0'. rewrite He'. rewrite Hcl.
+      simpl.
+      specialize (Henvo x).
+      destruct (envo x); simpl...
+      exfalso...
+    - specialize (to_cexp_complete _ H1) as [e' He'].
+      inv Hfind. destruct H2 as [cl Hcl].
+      eexists; simpl.
+      destruct e; try (rewrite Hcl; rewrite He'; simpl; eauto).
+      inv He'.
+      inv He'.
+  Qed.
+
+  Corollary mmap_to_equation_complete : forall eqs out env envo,
+      Forall (normalized_equation out) eqs ->
+      Forall (fun x => exists cl, find_clock env x = OK cl) (vars_defined eqs) ->
+      (forall x e, envo x = Error e -> In x out) ->
+      exists eqs', mmap (to_equation env envo) eqs = OK eqs'.
+  Proof.
+    induction eqs; intros out env envo Hnorm Hfind Henvo; simpl.
+    - eexists; eauto.
+    - inv Hnorm. destruct a.
+      simpl in Hfind. rewrite Forall_app in Hfind. destruct Hfind as [Hfind1 Hfind2].
+      specialize (to_equation_complete _ _ _ _ _ H1 Hfind1 Henvo) as [eq' Heq'].
+      eapply IHeqs in H2; eauto. destruct H2 as [eqs' Heqs'].
+      rewrite Heqs'; rewrite Heq'; eexists; simpl; eauto.
+  Qed.
+
+  Corollary mmap_to_equation_complete' : forall n out env envo,
+      Forall (normalized_equation out) (n_eqs n) ->
+      Forall (fun x => exists cl, find_clock env x = OK cl) (vars_defined (n_eqs n)) ->
+      (forall x e, envo x = Error e -> In x out) ->
+      exists eqs', mmap_to_equation env envo n = OK eqs'.
+  Proof.
+    intros n out env envo Hnorm Hfind Henvo.
+    eapply mmap_to_equation_complete in Hnorm; eauto.
+    destruct Hnorm as [eqs' Heqs'].
+    exists (exist (fun neqs : list NL.equation => _) eqs' Heqs').
+    unfold mmap_to_equation. rewrite Heqs'. reflexivity.
+  Qed.
+
+  Lemma to_node_complete : forall n,
+      normalized_node n ->
+      exists n', to_node n = OK n'.
+  Proof.
+    intros n Hnorm.
+    unfold to_node.
+    edestruct mmap_to_equation_complete' as [[? ?] H].
+    4: (rewrite H; eauto).
+    - unfold normalized_node in Hnorm. eassumption.
+    - specialize (n_defd n) as Hperm.
+      rewrite Forall_forall. intros x Hin.
+      eapply Permutation.Permutation_in in Hperm; eauto. clear Hin.
+      rewrite in_map_iff in Hperm; destruct Hperm as [[? [? ?]] [? Hin]]; simpl in H; subst.
+      erewrite envs_eq_find with (ck:=c); simpl; eauto.
+      + apply envs_eq_node.
+      + rewrite In_idck_exists.
+        exists t. repeat rewrite in_app_iff in *.
+        destruct Hin; auto.
+    - intros x e Hmem; simpl in Hmem.
+      rewrite <- fst_InMembers. rewrite <- Env.In_from_list.
+      apply Env.mem_2.
+      destruct (Env.mem x (Env.from_list (n_out n))); congruence.
+  Qed.
+End COMPLETENESS.
+
+Module CompletenessFun
+       (Ids : IDS)
+       (Op : OPERATORS)
+       (OpAux : OPERATORS_AUX Op)
+       (Str  : COINDSTREAMS Op OpAux)
+       (LSyn : LSYNTAX Ids Op)
+       (LTyp : LTYPING Ids Op LSyn)
+       (LOrd : LORDERED Ids Op LSyn)
+       (LSem : LSEMANTICS Ids Op OpAux LSyn LOrd Str)
+       (LNorm : LNORMALIZATION Ids Op OpAux Str LSyn LTyp LOrd LSem)
+       (CE : CESYNTAX Op)
+       (NL : NLSYNTAX Ids Op CE)
+       (TR : TRANSCRIPTION Ids Op OpAux LSyn CE NL)
+       <: COMPLETENESS Ids Op OpAux Str LSyn LTyp LOrd LSem LNorm CE NL TR.
+  Include COMPLETENESS Ids Op OpAux Str LSyn LTyp LOrd LSem LNorm CE NL TR.
+End CompletenessFun.
